Other Things
=======

Partial Fractions
-------

The technique of partial fractions come up in many areas in mathematics including the integration of rational functions and finding inverse Laplace Transforms (in differential equations).  An example is if we have the following rational function:
$$R(x)=\frac{2x-2}{x^2+4x+3}$$
and if we wish to write it as the sum of two simpler forms:
$$\frac{4}{x+3}-\frac{2}{x+1}$$

The technique of going from a general rational function to a sum of simpler rational functions is called *partial fractions*.  To do this, we recognize that if we factor the denomiator of $R$ or $(x+3)(x+1)$ so we hope to write:
$$\frac{2x-2}{x^2+4x+3} =\frac{A}{x+3}+\frac{B}{x+1}$$
or finding $A$ and $B$.  Multiplying through by the denominator of $R$ results in
$$2x-2 = A(x+1)+B(x+3)$$
or
$$2x-2=Ax+Bx+A+3B$$

at this point we *equate coefficients*  by finding the coefficients of the $x$ term and the constant term on either side of the equation. This results in two equations:
$$\begin{array}{rl}2&=A+B\\-2&=A+3B\end{array}$$

subtracting these, results in $4=-2B$ or $B=-2$ and then you can find $A=4$.  This shows that

$$\frac{2x-2}{x^2+4x+3}=\frac{4}{x+3}-\frac{2}{x+1}$$

###Using Maple to help us find partial fractions

We start again with 
```
R:=(2x-2)/(x^2+4x+3)
```

and we factor the denominator:

```
factor(denom(R))
```

returns $(x+3)(x+1)$, so we write the equation:
$$\frac{2x-2}{x^2+4x+3}=\frac{A}{x+3}+\frac{B}{x+1}$$
and then we multiply through by the denominator of $R$.
```
simplify((#)*denom(R))
```

where (#) is the equation above.  This returns:
$$2x-2 = Ax+Bx+A+3B$$

To get the equations representing the coefficients:
```
coeff(lhs((#)), x) = coeff(rhs((#)), x)
```

will return $2=A+B$, the coefficients of the $x$ terms on both sides.  To get the constant terms:
```
coeff(lhs((#)), x,0) = coeff(rhs((#)), x,0)
```

will return $-2=A+3B$. 

Lastly, we can just solve this to get: $\{A = 4, B = -2\}$ so the result is:

$$\frac{2x-2}{x^2+4x+3}=\frac{4}{x+3}-\frac{2}{x+1}$$

###Converting an expanded form back.  

How do you reverse the partial fraction?  If you are doing it by hand, it is simply finding a common denominator and combining terms.  In Maple, 
```
normal(4/(x+3)-2/(x+1),expanded)
```

returns $$\frac{2x-2}{x^2+4x+3}$$.


###Exercise 

Find the partial fraction form of
$$\frac{9x^2+8x-4}{x^3-4x}$$
using the steps above. Check your answer by reversing the partial fraction form.  


###Using the built-in method

Of course, Maple can do all of these steps at once.  If we use the $R$ from above, typing
```
convert(R,parfrac)
```

returns $$\frac{4}{x+3}-\frac{2}{x+1}.$$


###Exercise

1. Use `convert` to check your result above.  
2. Find the partial fraction form of $${\frac {4\,{x}^{6}+15\,{x}^{5}+34\,{x}^{4}+66\,{x}^{3}+94\,{x}^{2}+56\,x+40}{{x}^{4}+2\,{x}^{3}+5\,{x}^{2}+8\,x+4}}$$





Complex Numbers
-------


Mandlebrot Set
-------